pulse/src/checker/Pulse.Soundness.Rewrite.fst
@@ -38,11 +38,9 @@ let rewrite_soundness
 							  (elab_comp c)) =
 		
 		let T_Rewrite _ p q p_typing equiv_p_q = d in
-		let rp = elab_term p in
-		let rq = elab_term q in
-		let rp_typing : RT.tot_typing _ rp vprop_tm =
+		let rp_typing : RT.tot_typing _ p vprop_tm =
 		  tot_typing_soundness p_typing in
-		let rq_typing : RT.tot_typing _ rq vprop_tm =
+		let rq_typing : RT.tot_typing _ q vprop_tm =
 		  tot_typing_soundness (let f, _ = vprop_equiv_typing equiv_p_q in
 				                      f p_typing) in
 		let d_stt_vprop_equiv =
