pulse/src/checker/Pulse.Soundness.VPropEquiv.fst
@@ -34,12 +34,11 @@ open Pulse.Checker.VPropEquiv
 let vprop_equiv_refl_type = 
   let var = 0 in
   let v = mk_name var in
-  let v_typ = elab_term tm_vprop in
-  mk_arrow (v_typ, R.Q_Explicit)
+  mk_arrow (tm_vprop, R.Q_Explicit)
            (RT.close_term (stt_vprop_equiv v v) var)
 
 let inst_vprop_equiv_refl #g #v
-                          (d:RT.tot_typing g v (elab_term tm_vprop))
+                          (d:RT.tot_typing g v tm_vprop)
   : GTot (pf:R.term &
           RT.tot_typing g pf (stt_vprop_equiv v v))
   = admit()
@@ -49,12 +48,11 @@ let vprop_equiv_sym_type =
   let v0 = mk_name var0 in
   let var1 = 1 in
   let v1 = mk_name var1 in
-  let v_typ = elab_term tm_vprop in
   mk_arrow 
-    (v_typ, R.Q_Implicit)
+    (tm_vprop, R.Q_Implicit)
     (RT.close_term
       (mk_arrow
-        (v_typ, R.Q_Implicit)
+        (tm_vprop, R.Q_Implicit)
         (RT.close_term 
           (mk_arrow
              (stt_vprop_equiv v0 v1, R.Q_Explicit)
@@ -62,8 +60,8 @@ let vprop_equiv_sym_type =
         var0)
             
 let inst_vprop_equiv_sym #g #v0 #v1
-  (d0:RT.tot_typing g v0 (elab_term tm_vprop))
-  (d1:RT.tot_typing g v1 (elab_term tm_vprop))
+  (d0:RT.tot_typing g v0 tm_vprop)
+  (d1:RT.tot_typing g v1 tm_vprop)
   (#pf:_)
   (deq:RT.tot_typing g pf (stt_vprop_equiv v0 v1))
   : GTot (pf:R.term &
@@ -71,9 +69,9 @@ let inst_vprop_equiv_sym #g #v0 #v1
   = admit()
 
 let inst_vprop_equiv_trans #g #v0 #v1 #v2
-                         (d0:RT.tot_typing g v0 (elab_term tm_vprop))
-                         (d1:RT.tot_typing g v1 (elab_term tm_vprop))
-                         (d2:RT.tot_typing g v2 (elab_term tm_vprop))
+                         (d0:RT.tot_typing g v0 tm_vprop)
+                         (d1:RT.tot_typing g v1 tm_vprop)
+                         (d2:RT.tot_typing g v2 tm_vprop)
                          (#pf01:_)
                          (d01:RT.tot_typing g pf01 (stt_vprop_equiv v0 v1))
                          (#pf12:_)                         
@@ -84,10 +82,10 @@ let inst_vprop_equiv_trans #g #v0 #v1 #v2
 
 
 let inst_vprop_equiv_cong #g #v0 #v1 #v0' #v1'
-                         (d0:RT.tot_typing g v0 (elab_term tm_vprop))
-                         (d1:RT.tot_typing g v1 (elab_term tm_vprop))
-                         (d0':RT.tot_typing g v0' (elab_term tm_vprop))
-                         (d1':RT.tot_typing g v1' (elab_term tm_vprop))                         
+                         (d0:RT.tot_typing g v0 tm_vprop)
+                         (d1:RT.tot_typing g v1 tm_vprop)
+                         (d0':RT.tot_typing g v0' tm_vprop)
+                         (d1':RT.tot_typing g v1' tm_vprop)
                          (#pf0:_)
                          (eq0:RT.tot_typing g pf0 (stt_vprop_equiv v0 v0'))
                          (#pf1:_)                         
@@ -98,24 +96,24 @@ let inst_vprop_equiv_cong #g #v0 #v1 #v0' #v1'
 
 
 let inst_vprop_equiv_unit #g #v
-                         (d:RT.tot_typing g v (elab_term tm_vprop))
+                         (d:RT.tot_typing g v tm_vprop)
   : GTot (pf:R.term &
-          RT.tot_typing g pf (stt_vprop_equiv (mk_star (elab_term tm_emp) v) v))
+          RT.tot_typing g pf (stt_vprop_equiv (mk_star tm_emp v) v))
   = admit()
 
 
 let inst_vprop_equiv_comm #g #v0 #v1
-                         (d0:RT.tot_typing g v0 (elab_term tm_vprop))
-                         (d1:RT.tot_typing g v1 (elab_term tm_vprop))                         
+                         (d0:RT.tot_typing g v0 tm_vprop)
+                         (d1:RT.tot_typing g v1 tm_vprop)
   : GTot (pf:R.term &
           RT.tot_typing g pf (stt_vprop_equiv (mk_star v0 v1) (mk_star v1 v0)))
   = admit()
 
 
 let inst_vprop_equiv_assoc #g #v0 #v1 #v2
-                         (d0:RT.tot_typing g v0 (elab_term tm_vprop))
-                         (d1:RT.tot_typing g v1 (elab_term tm_vprop))                         
-                         (d2:RT.tot_typing g v2 (elab_term tm_vprop))                                                  
+                         (d0:RT.tot_typing g v0 tm_vprop)
+                         (d1:RT.tot_typing g v1 tm_vprop)
+                         (d2:RT.tot_typing g v2 tm_vprop)
   : GTot (pf:R.term &
           RT.tot_typing g pf (stt_vprop_equiv (mk_star v0 (mk_star v1 v2)) (mk_star (mk_star v0 v1) v2)))
   = admit()
@@ -191,7 +189,7 @@ let rec vprop_equiv_soundness (#g:stt_env) (#v0 #v1:term)
   : GTot (pf:R.term &
           RT.tot_typing (elab_env g)
                         pf
-                        (stt_vprop_equiv (elab_term v0) (elab_term v1)))
+                        (stt_vprop_equiv v0 v1))
          (decreases eq)
   = match eq with
     | VE_Refl _ _ ->
@@ -258,15 +256,15 @@ let rec vprop_equiv_soundness (#g:stt_env) (#v0 #v1:term)
 #pop-options
 
 let stt_vprop_equiv_is_prop (#g:R.env) (#v0 #v1:R.term)
-                            (d0: RT.tot_typing g v0 (elab_term tm_vprop))
-                            (d1: RT.tot_typing g v1 (elab_term tm_vprop))
+                            (d0: RT.tot_typing g v0 tm_vprop)
+                            (d1: RT.tot_typing g v1 tm_vprop)
    : GTot (RT.tot_typing g (stt_vprop_equiv v0 v1) RT.tm_prop)
    = admit()
    
 let vprop_equiv_unit_soundness (#g:stt_env) (#v0 #v1:term) 
                                (d0:tot_typing g v0 tm_vprop)
                                (eq:vprop_equiv g v0 v1)
-  : GTot (RT.tot_typing (elab_env g) (`()) (stt_vprop_equiv (elab_term v0) (elab_term v1)))
+  : GTot (RT.tot_typing (elab_env g) (`()) (stt_vprop_equiv v0 v1))
   = let (| pf, s |) = vprop_equiv_soundness d0 eq in
     let d1 = fst (vprop_equiv_typing eq) d0 in
     let s_prop = stt_vprop_equiv_is_prop (tot_typing_soundness d0) (tot_typing_soundness d1) in
