pulse/src/checker/Pulse.Soundness.While.fst
@@ -43,7 +43,7 @@ let while_soundness
                         (elab_comp c)) =
 
   let T_While _ inv cond body inv_typing cond_typing body_typing = d in
-  let rinv = mk_abs bool_tm R.Q_Explicit (elab_term inv) in
+  let rinv = mk_abs bool_tm R.Q_Explicit inv in
   let rinv_typing
     : RT.tot_typing _
         (mk_exists uzero bool_tm rinv)
@@ -70,10 +70,10 @@ let while_soundness
     let d = soundness g body (comp_while_body ppname_default inv) body_typing in
     let pre_eq : RT.equiv (elab_env g)
                           (R.pack_ln (R.Tv_App rinv (true_tm, R.Q_Explicit)))
-                          (RT.subst_term (elab_term inv) [ RT.DT 0 true_tm ])
-      = assume (RT.ln' (elab_term inv) 0);
+                          (RT.subst_term inv [ RT.DT 0 true_tm ])
+      = assume (RT.ln' inv 0);
         assume (RT.ln true_tm);
-        RT.Rel_beta _ bool_tm R.Q_Explicit (elab_term inv) true_tm  in
+        RT.Rel_beta _ bool_tm R.Q_Explicit inv true_tm  in
     RT.T_Sub _ _ _ _ d
       (RT.Relc_typ _ _ _ _ _
          (RT.Rel_equiv _ _ _ _
@@ -84,9 +84,9 @@ let while_soundness
 
   let post_eq : RT.equiv (elab_env g)
     (RT.mk_abs unit_tm R.Q_Explicit
-       (R.pack_ln (R.Tv_App (mk_abs bool_tm R.Q_Explicit (elab_term inv)) (false_tm, R.Q_Explicit))))
+       (R.pack_ln (R.Tv_App (mk_abs bool_tm R.Q_Explicit inv) (false_tm, R.Q_Explicit))))
     (RT.mk_abs unit_tm R.Q_Explicit
-       (RT.subst_term (elab_term inv) [ RT.DT 0 false_tm ]))
+       (RT.subst_term inv [ RT.DT 0 false_tm ]))
     = RU.magic () in
 
   let d = WT.while_typing rinv_typing rcond_typing rbody_typing in
